\documentclass[a4paper]{article}
\usepackage[left=3.5cm, right=2.5cm, top=2.5cm, bottom=2.5cm]{geometry}
\usepackage[MeX]{polski}
\usepackage[utf8]{inputenc}
\usepackage{graphicx}
\usepackage{enumerate}
\usepackage{amsmath} %pakiet matematyczny
\usepackage{amssymb} %pakiet dodatkowych symboli
\begin{document}
$$ \sqrt{ \frac{2^{n}}{2_n}} \neq \sqrt[\frac{1}{3}]{1+n} $$

$$ \frac{2^{k}}{2^{k+2}} $$

$$ \frac{x^{2}}{2^{(x+2)(x-2)^{2}}} $$

$$ \log_{2} 2^{8} = 8 $$

$$ \sqrt[3]{e^{x}-log_{2}x} $$

$$ \lim_{x \to \infty} \sum_{k=1}^{n} \frac{1}{k^{2}} = \frac{\pi^{2}}{6} $$

$$ \int_{2}^{\infty} \frac{1}{log_{2}x}dx = \frac{1}{x} \sin{x} = 1 - \cos^{2}{(x)} $$

$$ \left[ \begin{array}{cccc}
a_{11} & a_{12} & \ldots & a_{1K} \\
a_{21} & a_{22} & \ldots & a_{2K} \\
\vdots & \vdots & \ddots & \vdots \\
a_{K1} & a_{K2} & \ldots & a_{KK} \\
\end{array} \right] 
*
\left[ \begin{array}{cccc}
x_{1} \\
x_{2} \\
\vdots \\
x_{K} \\
\end{array} \right]
=
\left[ \begin{array}{cccc}
b_{1} \\
b_{2} \\
\vdots \\
b_{K} \\
\end{array} \right]
$$

$$ (a_{1} = a_{1}(x)) \wedge (a_{2} = a_{2}(x)) \wedge \ldots \wedge (a_{k}= a_{k}(x)) \Rightarrow (d = d (u))  $$

$$  [x]_{A} = \left\lbrace y \in U : a (x) = a (y), \forall{a} \in A \right\rbrace , \ where \ the \ control \ object \ x \in U  $$

$$ T:[0,1] \times [0,1] \rightarrow [0,1] $$

$$ \lim_{x \to \infty} \exp (-x) = 0 $$

$$ \frac{n!}{k! (n-k)!} = {n \choose k}  $$

$$ P \left( A = 2 \bigg| \frac{A^{2}}{B} > 4 \right) $$

$$ S^{C_{i}}(a) = \frac{(\overline{C}_{i}^{a} - \hat{C}_{i}^{a})^{2}}{Z_{{\overline{C}_{i}^{a}}^{2}} + Z_{{\hat{C}_{i}^{a2}}}} , a \in A  $$

$$ \begin{cases}
|z| = |z-4i| \\
\frac{\pi}{4} \geq \arg{z} < \frac{\pi}{2} 
\end{cases} $$

$$ \begin{cases}
|z+4| = |z+2-2i| \\
|z| \geq 2
\end{cases} $$

$$ \begin{cases}
|z-1-i| < \sqrt{2} \\
\arg{(z-1-i)} < \frac{\pi}{2} 
\end{cases} $$

$$ \begin{cases}
\ x \ + \ 5y \ = \ 2 \\
-3x \ + \ 6y \ = \ 15
\end{cases} $$

$$ \begin{cases}
\ x \ - \ y \ - \ z \ = \ 1 \\
\ 3x \ + \ 4y \ - \ 2z \ = \ -1 \\
\ 3x \ - \ 2y \ - \ 2z \ = \ 1
\end{cases} $$

$$ \begin{cases}
\ y \ - \ 3z \ + \ 4v \ = \ 0 \\
\ x \ - \ 2z \ = \ 0 \\
\ 3x \ + \ 2y \ - \ 5v \ = \ 2 \\
\ 4x \ - \ 5z \ = \ 0
\end{cases} $$

\end{document}